proof/refine/X64/CNodeInv_R.thy
@@ -656,7 +656,7 @@ lemma prepareThreadDelete_not_recursive_ctes:
   "\<lbrace>\<lambda>s. P (not_recursive_ctes s)\<rbrace>
      prepareThreadDelete t
    \<lbrace>\<lambda>rv s. P (not_recursive_ctes s)\<rbrace>"
-  by (wpsimp simp: prepareThreadDelete_def fpuThreadDelete_def not_recursive_ctes_def cteCaps_of_def)
+  by (wpsimp simp: prepareThreadDelete_def not_recursive_ctes_def cteCaps_of_def)
 
 definition
   finaliseSlot_recset :: "((machine_word \<times> bool \<times> kernel_state) \<times> (machine_word \<times> bool \<times> kernel_state)) set"
@@ -9014,7 +9014,6 @@ crunch finaliseCap
   (wp: crunch_wps unless_wp getASID_wp no_irq
        no_irq_writeCR3 no_irq_invalidateASID
        no_irq_invalidateLocalPageStructureCacheASID
-       no_irq_switchFpuOwner no_irq_nativeThreadUsingFPU
    simp: crunch_simps o_def)
 
 lemma finaliseSlot_IRQInactive':
